\chapter{The Universal Enveloping Algebra}


\begin{convention}
  The following holds for this section alone:
  We fix an arbitrary field~$\kf$.
  By a~{\algebra{$\kf$}} we always mean an associative and unitary one, and homomorphisms of~{\algebras{$\kf$}} have to respect the units.
  The resulting category of~{\algebras{$\kf$}} with homomorphisms of~{\algebra{$\kf$}} between them will be denoted by~$\cAlg{\kf}$.
  All Lie~algebras considered will have~$\kf$ as their ground field, unless otherwise stated.
  
  If~$A$ is a~{\algebra{$\kf$}} then by an~\defemph{\module{$A$}}\index{module} we mean a left unitial~{\module{$A$}}.
  The resulting category of~{\modules{$A$}} is denoted by~\gls*{module category}.
\end{convention}




\input{sections/tensor_algebra_and_symmetric_algebra}
\input{sections/definition_and_construction_of_the_uea}
\input{sections/the_pbw_theorem}


% TODO: Hopf algebra structure
% TODO: Casimir elements

% 
% 
% 
% 
% 
% 
% \section{Casimir elements}
% For this subsection we additionaly assume that $\glie$ is finite-dimensional. We also fix some bilinear form $\beta \colon \glie \times \glie \to k$ which is associative and non-degenerate.
% 
% 
% \begin{definition}\label{defi: definition of Casimir element}
%  Let $\varphi_1 \colon \glie \tensor \g^* \to \End_k(\g)$ and $\varphi_2 \colon \glie \to \g^*$ be the isomorphisms of vector spaces defined by
%  \[
%   \varphi_1(x \tensor \phi)(y) = \phi(y) x
%   \quad\text{and}\quad
%   \varphi_2(x) = \beta(x, \cdot)
%   \quad\text{for all $x,y \in \g$ and $\phi \in \g^*$}.
%  \]
%  Then the image of $1$ under the map
%  \begin{equation}\label{eqn: Casimir without coordinates}
%   k
%   \xrightarrow{\lambda \mapsto \lambda \id_\g}
%   \End_k(\g)
%   \xrightarrow{\varphi_1^{-1}}
%   \glie \tensor \g^*
%   \xrightarrow{\id_\g \tensor \varphi_2^{-1}}
%   \glie \tensor \g
%   \xrightarrow{x \tensor y \mapsto x y}
%   \Univ(\glie)
%  \end{equation}
%  is called the \emph{Casimir element of $\beta$} and denoted by $C_\beta$.
% \end{definition}
% 
% 
% \begin{lemma}
%  The Casimir element $C_\beta$ in central in $\Univ(\glie)$, i.e.\
%  \[
%   x C_\beta = C_\beta x \quad \text{for every $x \in \Univ(g)$}.
%  \]
% \end{lemma}
% \begin{proof}
%  Let $\varphi_1$ and $\varphi_2$ as in Definition \ref{defi: definition of Casimir element}.
%  
%  Because $\Univ(\glie)$ is generated by $\glie$ as a \algebra{$\kf$} it sufficies to show $C_\beta$ commutes with every $x \in \g$. Hence it is to show that
%  \[
%   [x,C_\beta] = 0 \quad \text{for every $x \in \g$},
%  \]
%  where $[\cdot,\cdot]$ denotes the Lie bracket in $\Univ(\glie)$. To see this notice that in \eqref{eqn: Casimir without coordinates} every map is a homomorphism of representations of $\glie$, where $\glie$ acts trivially on $k$, i.e. $x.\lambda = 0$ for every $x \in \g$ and $\lambda \in \g$.
%  
%  That the first map $k \to \End_k(\g)$ is a homomorphism of representations follows from the fact that $\glie$ acts trivially on $k$ and also trivially on the one-dimensional subspace $k \id_\g \subseteq \End_k(\g)$.
%  
%  That $\varphi_1$ is an isomorphism of representations is known from Propositon \ref{prop: list of homomorphism of representations}.
%  
%  That the third map $\glie \tensor \g^* \to \glie \tensor \g$ is a homomorphism of representations follows from Proposition \ref{prop: list of homomorphism of representations}, because the identity $\id_\g$ is a homomorphism of representations and and the isomorphism $\varphi_2$ is one by the associativity of $\beta$, as seen in Lemma \ref{lem: associative bilinear form induces homomorphism of representations}.
%  
%  That the fourth map $\psi \colon \glie \tensor \glie \to \Univ(\glie), x \tensor y \mapsto xy$ is a homomorphism of representations follows from direct calculation, because for all $x,y,z \in \g$
%  \begin{align*}
%   \psi(x.(y \tensor z))
%   &= \psi((x.y) \tensor z + y \tensor (x.z))
%   = (x.y)z + y(x.z) \\
%   &= [x,y]z + y[x,z]
%   = xyz - yxz + yxz - yzx
%   = xyz - yzx \\
%   &= [x,yz]
%   = x.(yz)
%   = x.\psi(y \tensor z).
%  \end{align*}
%  
%  Because every map in \eqref{eqn: Casimir without coordinates} is a homomorphism of representations it follows that their composition $\phi \colon k \to \Univ(\glie)$ is also a homomorphism of representations. Definition \ref{defi: definition of Casimir element} is then equivalent to $\phi(1) = C_\beta$. Because $\glie$ acts trivially on $k$ and $\phi$ is a homomorphism of representations it follows that $\glie$ also acts trivially on the span of $C_\beta$. In particular
%  \[
%   0 = x.C_\beta = [x,C_\beta] \quad \text{for every $x \in \g$}.
%   \qedhere
%  \]
% \end{proof}
% 
% 
% \begin{corollary}\label{cor: Casimir homomorphism of a representation}
%  Let $V$ be a representation of $\glie$ and $\Univ(\glie) \times V \to V, (x,v) \mapsto x \cdot v$ the corresponding $\Univ(\glie)$-module structure on $V$. Then the map
%  \[
%   C_\beta^V \colon V \to V, \quad v \mapsto C_\beta \cdot v = \sum_{i=1}^n x_i.x^i.v
%  \]
%  is an endomorphism of representations of $\glie$ (equivalently an endomorphism of $\Univ(\glie)$-modules).
% \end{corollary}
% \begin{proof}
%  Because $C_\beta \in Z(\Univ(\glie))$ it follows that for every $x \in \Univ(\glie)$ and $v \in V$
%  \[
%   x \cdot C_\beta^V(v)
%   = x \cdot C_\beta \cdot v
%   = C_\beta \cdot x \cdot v
%   = C_\beta^V(x \cdot v).
%   \qedhere
%  \]
% \end{proof}
% 
% 
% \begin{lemma}[Casimir in coordinates] \label{lem: casimir in coordinates}
%  Let $x_1, \dotsc, x_n$ be a basis of $\glie$ and $x^1, \dotsc, x^n$ the dual basis of $\glie$ with respect to $\beta$, i.e.\ $\beta(x_i, x^j) = \delta_{ij}$ for all $i,j = 1, \dotsc, n$. Then
%  \[
%   C_\beta = \sum_{i=1}^n x_i x^i.
%  \]
% \end{lemma}
% \begin{proof}
%  Let $\varphi_1$ and $\varphi_2$ as in Definition~\ref{defi: definition of Casimir element}. In \eqref{eqn: Casimir without coordinates} $1$ is mapped to $\id_\g$, which is then mapped to $\sum_{i=1}^n x_i \tensor x_i^*$, where $x_1^*, \dotsc, x_n^*$ denotes the dual basis of $\g^*$. As $\varphi_2(x^i) = x_i^*$ it follows that $\sum_{i=1}^n x_i \tensor x_i^*$ is then mapped to $\sum_{i=1}^n x_i \tensor x^i$, which is then further mapped to the element $\sum_{i=1}^n x_i x^i$ in $\Univ(\glie)$.
% \end{proof}
% 
% 
% \begin{remark}
%  Using Lemma \ref{lem: casimir in coordinates} it can be shown that $C_\beta$ is central in $\Univ(\glie)$ using coordinates: Let $x \in \g$ and $a_{ij}, b_{ij} \in k$ such that $[x,x_i] = \sum_{j=1}^n a_{ij} x_j$ and $[x,x^i] = \sum_{j=1}^n b_{ij} x^j$ for all $i = 1, \dotsc, n$. Then for all $i,j = 1, \dotsc, n$
%  \begin{align*}
%   a_{ij}
%   &= \sum_{k=1}^n a_{ik} \beta(x_k, x^j)
%   = \beta\left( \sum_{k=1}^n a_{ik} x_k, x^j \right)
%   = \beta([x, x_i], x^j)
%   = -\beta([x_i, x], x^j) \\
%   &= -\beta(x_i, [x, x^j])
%   = -\beta\left( x_i, \sum_{k=1}^n b_{jk} x^k \right)
%   = -\sum_{k=1}^n b_{jk} \beta(x_i, x^k)
%   = -b_{ji}.
%  \end{align*}
%  It follows that
%  \begin{align*}
%   x C_\beta - C_\beta x
%   &= \sum_{i=1}^n x x_i x^i - \sum_{i=1}^n x_i x^i x
%   = \sum_{i=1}^n [x, x_i] x^i - \sum_{i=1}^n x_i [x^i, x] \\
%   &= \sum_{i,j=1}^n a_{ij} x_j x^i + \sum_{i,j=1}^n b_{ij} x_i x^j
%   = \sum_{i,j=1}^n a_{ij} x_j x^i - \sum_{i,j=1}^n a_{ij} x_j x^i
%   = 0.
%  \end{align*}
% \end{remark}




